---
title:  "A First-Order Non-Linear PDE with a well-defined Complete Integral & General Integral"
date:   2022-01-11 16:35:42 +0100
categories: pde math maple 
---

This post will be dedicated to: 

$$\begin{equation} \tag{$1$}\label{1}
u_x^2 + u_y^2 + u = 1
\end{equation}$$  

The PDE possesses a well defined envelope solution (general integral), on top of its complete integral. It's a visually appealling case, since if the method that we are going to use was forced on a similar nonlinear first order PDE in the similar form of $$ F(u,u_x,u_y) = 0$$, such as $$ u_x^4 + u_y^4 + u = 1 $$, or $$ u_x^4 + u_y^4 -u^3 = 0 $$, it would be seen that resulting general integral is a fraction of x and y which is not well defined, and hence not as much of a visually appealling plot such as this PDE.

## Solving Method 

1. Obtain Charpit Equations
2. Obtain relationship between $$p$$ and $$q$$, where $$p$$,$$q$$ are shorthand for $$u_x$$,$$u_y$$, respectively.
3. Using the relationship obtained in step 2, sub into the original PDE to get $$p$$ & $$q$$ in terms of u.
3. Use the chainrule $$\frac{du}{dt} = u_x\frac{dx}{dt} + u_y\frac{dy}{dt}$$, substitute p and q, integrate, and rearrange for u. This is the Complete Integral(CI) solution.
4. Differentiate the CI w.r.t to the constant obtained in step 2. Rearrange for the constant. Sub it into the CI to obtain the envelope solution.

### Steps 1 & 2

The only relevant Charpit's equations needed here are $$\frac{dp}{-p}=\frac{dq}{-q}$$. Following the standard procedures for integrating:-

$$\frac{dp}{p}=\frac{dq}{q} \implies \ln(p) = \ln(q) + c \implies p = \alpha q$$, where $$\alpha$$ is a constant.

### Step 3

Subbing $$ p = \alpha q$$ into $$\eqref{1}$$, we get:-

$$\alpha^2q^2 +q^2 +u - 1 =0 \implies q^2 = \frac{1-u}{1+\alpha^2}\implies q = \pm\sqrt{\frac{1-u}{1+\alpha^2}}$$


Subbing $$ q = \frac{p}{\alpha}$$ into $$\eqref{1}$$, we get:-

$$p^2+\frac{p^2}{\alpha^2}+u-1=0 \implies p^2 = \frac{\alpha^2-u\alpha^2}{\alpha^2+1}\implies p=\pm\sqrt{\frac{\alpha^2-u\alpha^2}{\alpha^2+1}}$$

### Step 4 (Taking the "positive" p & q)



$$\begin{align}
&\frac{du}{dt} = \sqrt{\frac{\alpha^2-u\alpha^2}{\alpha^2+1}}\frac{dx}{dt}+\sqrt{\frac{1-u}{1+\alpha^2}}\frac{dy}{dt} \\
(1-u)^\frac{-1}{2}&\frac{du}{dt} = \frac{1}{\sqrt{1+\alpha^2}}\frac{dx}{dt} + \frac{\alpha}{\sqrt{1+\alpha^2}}\frac{dy}{dt}\\
&(1-u)^\frac{1}{2} = \frac{-1}{2}\frac{x+\alpha y + \beta}{\sqrt{1+\alpha^2}}\\
&u= 1 - \frac{(\alpha x +y+\beta)^2}{4(1+\alpha^2)^2} \tag{2}\label{2}
\end{align}$$  

which is a family of solutions to the PDE $$\eqref{1}$$.



### Step 5

Differentiating $$\eqref{2}$$ w.r.t. $$\alpha$$, we get:

$$ \frac{(\alpha x + y + \beta)(\alpha y + \alpha \beta - x)}{2(1+\alpha^2)^2} = 0 $$

Rearranging for $$\alpha$$, we get:  

$$\alpha_1 = -\frac{y+\beta}{x}$$  
$$\alpha_2 = \frac{x}{y+\beta}$$  

$$\alpha_1$$ gives a trivial solution, but subbing $$\alpha_2$$ gives the desired family of solutions:-  
$$\begin{equation} \tag{3}\label{3}
u = 1 - \frac{x^2}{4} - \frac{(y+\beta)^2}{4}
\end{equation}$$  

## Observing the solution

We can fix the constant $$\beta$$ in both $$\eqref{2}$$ and $$\eqref{3}$$, and vary the $$\alpha$$ in $$\eqref{2}$$, to visually understand why $$\eqref{3}$$ is an "envelope" solution.  

Let's fix $$\beta = 0$$, $$u = 0$$ and vary $$\alpha$$ between -5 & 5, and plot both solutions on an x-y plane.

![Combined plot](/assets/images/PDEs2/comb_plot.png){: .full}

which can be achieved with the Maple Code
~~~
with(plots):
A := implicitplot(1 - x^2/4 - y^2/4 = 0, x = -5 .. 5, y = -5 .. 5, color = red):
B := implicitplot([seq(1 - (alpha*x + y)^2/(4*(alpha^2 + 1)^2), alpha = -5 .. 5, 0.25)], x = -5 .. 5, y = -5 .. 5, colour = blue):
display([A, B])
~~~  