---
title:  "Analysing a Travelling Wave Solution of a PDE with an Initial Condition"
date:   2022-01-07 19:35:42 +0100
categories: pde math maple 
---
## The problem

$$\begin{align}
&u_t + u^2u_x = 0 \\
&u(x,0) = sech(x)
\end{align}$$

The PDE is not directly solveable via integration, so we will resort to the method of characteristics.
## GS and characteristics

It can be shown that the general solutions to a PDE of the form:

$$\begin{equation} \tag{1a}\label{eqn1}
u_t + c(u)u_x = 0
\end{equation}$$  

$$\begin{equation} \tag{1b}\label{ic}
u(x,0) = f(x)
\end{equation}$$

have solutions that adhere to the same form. 

Firstly, we can use the chain rule $$\frac{du}{dt} = u_t + \frac{dx}{dt}u_x$$. We can observe that it follows the form of $$\eqref{eqn1}$$ and hence: $$\frac{du}{dt} = 0 \Rightarrow u = w$$ , where w is a constant.    

Next, we use the parametrised method of characteristics to obtain the simultaneous equations:

$$\begin{equation} \tag{2a}\label{eqn3}
\frac{dt}{ds} = 1
\end{equation}$$  
$$\begin{equation} \tag{2b}\label{eqn4}
\frac{dx}{ds} = c(u)
\end{equation}$$ 

& from this we can show that: 

$$\begin{equation}
c(u)\frac{dt}{ds} \stackrel{c(u)\eqref{eqn3}=\eqref{eqn4}}= \frac{dx}{ds} 
\end{equation}$$

$$\begin{equation} \tag{3}\label{eqn5}
x = c(u)t + \xi \implies x = c(w)t + \xi
\end{equation}$$

$$\begin{equation} \tag{4}\label{eqn6}
\therefore u = w(\xi) \implies u=w(x-c(w)t)
\end{equation}$$

Note that the characteristics are given by the equation $$\eqref{eqn5}$$. Also note that at t = 0 we have that $$\eqref{eqn5}$$ turns into $$ x = \xi $$.

$$ u(x,0) = f(x) \implies w(x)=f(x) \implies w(\xi) = f(\xi)$$  
$$ \therefore u = f(x-tc(u)) $$. $$\eqref{eqn6}$$.

We can now summarise this. A PDE of the form $$u_t + c(u)u_x = 0$$ has the characteristics $$x = c(u)t + \xi$$ $$\eqref{eqn5}$$ and a general solution of the form $$u=f(\xi)=f(x-c(u)t)$$, which is a travelling wave solution.

## Back to the original problem
